EventStructure.v
@@ -37,15 +37,13 @@ Definition thread_id l :=
 (*     Exec Event Structure                                                         *)
 (* ******************************************************************************** *)
 
+
 Structure exec_event_struct := Pack {
   n     : nat;
   lab   : 'I_n -> label;
   fpred : forall m : 'I_n, option 'I_m;
-  frf   : forall r : 'I_n, 
-            { w :? 'I_r | 
-                 (opred is_read \o ext lab) r 
-              |- (orel compatible \o2 ext lab) w r 
-            } 
+  frf   : forall (r : 'I_n) (is_r : (opred is_read \o ext lab) r), 
+            { w : 'I_r | (orel compatible \o2 ext lab) w r } 
 }.
 
 Section ExecEventStructure.
@@ -57,6 +55,9 @@ Notation lab     := (lab es).
 Notation fpred   := (fpred es).
 Notation frf     := (frf es).
 Notation ltn_ind := (@ltn_ind n).
+
+(* Definition TT (r : nat) : Type := *)
+(*   forall (_ : (opred is_read \o ext lab) r), { w : 'I_r | (orel compatible \o2 ext lab) w r }. *)
 
 (* ******************************************************************************** *)
 (*     Event Types                                                                  *)
@@ -92,26 +93,26 @@ Proof. rewrite /succ. by move /eqP /ofpred_lt. Qed.
 (*     Reads-From                                                                   *)
 (* ******************************************************************************** *)
 
-(* Definition ofrf (e : 'I_n) : option 'I_n := *)
-(*   omap *)
-(*     (fun r => *)
-(*        let rv : 'I_n := sval   r in *)
-(*        let rpf := opred_ext is_read lab rv (sproof r) in *)
-(*        advance rv (sval (frf rv rpf)) *)
-(*     ) *)
-(*     (oread e). *)
-
 Definition ofrf (e : 'I_n) : option 'I_n :=
-  omap (advance e) (sval (frf e)).
+  omap
+    (fun r =>
+       let rv : 'I_n := sval   r in
+       let rpf := opred_ext is_read lab rv (sproof r) in
+       advance rv (sval (frf rv rpf))
+    )
+    (oread e).
+
+(* Definition ofrf (e : 'I_n) : option 'I_n := *)
+(*   omap (advance e) (sval (frf e)). *)
 
 Lemma ofrf_le r w : ofrf r = some w -> w < r.
 Proof.
   rewrite /ofrf /oread.
-  case: (sval (frf r)) => [x [<-]|] //=.
-  (* case b: (is_read (lab r)); first last. *)
-  (* { by rewrite insubF. } *)
-  (* rewrite insubT//= => [[<-]]/=. *)
-  (* exact: ltn_ord.  *)
+  (* case: (sval (frf r)) => [x [<-]|] //=. *)
+  case b: (is_read (lab r)); first last.
+  { by rewrite insubF. }
+  rewrite insubT//= => [[<-]]/=.
+  exact: ltn_ord.
 Qed.
 
 (* Reads-From relation *)
